src/Spec/Compile.v
@@ -1,0 +1,223 @@
+Require Import ConcurProc.
+Require Import Equiv.
+Require Import Helpers.Helpers.
+Require Import FunctionalExtensionality.
+
+Global Set Implicit Arguments.
+Global Generalizable All Variables.
+
+
+Section Compiler.
+
+  Variable opLoT : Type -> Type.
+  Variable opMidT : Type -> Type.
+  Variable opHiT : Type -> Type.
+
+  Variable compile_op : forall T, opMidT T -> proc opLoT opMidT T.
+
+  Definition atomize {T} (op : opMidT T) : proc opLoT opMidT T :=
+    Atomic (compile_op op).
+
+  Definition hicall T (op : opMidT T) : proc opLoT opMidT T :=
+    _ <- OpCallHi op;
+    r <- compile_op op;
+    OpRetHi r.
+
+  Inductive compile_ok : forall T (p1 : proc opLoT opMidT T) (p2 : proc opMidT opHiT T), Prop :=
+  | CompileOpcode : forall `(op : opMidT T),
+    compile_ok (hicall op) (Op op)
+  | CompileRet : forall `(x : T),
+    compile_ok (Ret x) (Ret x)
+  | CompileBind : forall `(p1a : proc opLoT opMidT T1) (p2a : proc opMidT opHiT T1)
+                         `(p1b : T1 -> proc _ _ T2) (p2b : T1 -> proc _ _ T2),
+    compile_ok p1a p2a ->
+    (forall x, compile_ok (p1b x) (p2b x)) ->
+    compile_ok (Bind p1a p1b) (Bind p2a p2b)
+  | CompileOpCallHi : forall `(op : opHiT T),
+    compile_ok (Ret tt) (OpCallHi op)
+  | CompileOpRetHi : forall `(v : T),
+    compile_ok (Ret v) (OpRetHi v).
+
+  Fixpoint compile T (p : proc opMidT opHiT T) : proc opLoT opMidT T :=
+    match p with
+    | Ret t => Ret t
+    | OpCall op => OpCallHi op
+    | OpExec op => compile_op op
+    | OpRet r => OpRetHi r
+    | Bind p1 p2 => Bind (compile p1) (fun r => compile (p2 r))
+    | OpCallHi _ => Ret tt
+    | OpRetHi v => Ret v
+    | Atomic p => Atomic (compile p)
+    end.
+
+End Compiler.
+
+Arguments hicall {opLoT opMidT} compile_op {T}.
+
+Hint Constructors compile_ok.
+
+
+Ltac destruct_ifs :=
+  repeat match goal with
+  | |- context[if ?a == ?b then _ else _] =>
+    destruct (a == b)
+  end.
+
+Section Disjoint.
+
+  Variable opT : Type -> Type.
+  Variable opHiT : Type -> Type.
+  Variable ThreadState : Type.
+  Definition State := forall (tid : nat), ThreadState.
+  Variable op_step : OpSemantics opT State.
+
+  Definition state_upd (s : State) (tid : nat) (val : ThreadState) :=
+    fun tid' =>
+      if tid' == tid then val else s tid'.
+
+  Theorem state_upd_upd_ne : forall tid1 v1 tid2 v2 s, tid1 <> tid2 ->
+    state_upd (state_upd s tid1 v1) tid2 v2 =
+    state_upd (state_upd s tid2 v2) tid1 v1.
+  Proof.
+    intros; apply functional_extensionality; intros.
+    unfold state_upd.
+      destruct_ifs; congruence.
+  Qed.
+
+  Theorem state_upd_ne : forall tid1 v1 tid2 s, tid1 <> tid2 ->
+    state_upd s tid1 v1 tid2 = s tid2.
+  Proof.
+    intros; unfold state_upd; destruct_ifs; congruence.
+  Qed.
+
+
+  Definition disjoint_writes := forall T (op : opT T) tid s v s',
+    op_step op tid s v s' ->
+    forall tid0,
+      tid0 <> tid ->
+      s tid0 = s' tid0.
+
+  Definition disjoint_reads := forall T (op : opT T) tid s v s',
+    op_step op tid s v s' ->
+    forall tid0 x,
+    tid0 <> tid ->
+    op_step op tid
+      (state_upd s tid0 x)
+      v
+      (state_upd s' tid0 x).
+
+  Variable disjoint_w : disjoint_writes.
+  Variable disjoint_r : disjoint_reads.
+
+  Lemma exec_tid_disjoint_writes : forall T tid0 s p s' result' evs,
+    @exec_tid opT opHiT State op_step T tid0 s p s' result' evs ->
+    forall tid1,
+      tid0 <> tid1 ->
+      s tid1 = s' tid1.
+  Proof.
+    intros.
+    induction H; eauto.
+    induction H; eauto.
+    + eapply eq_trans.
+      apply IHatomic_exec1; eauto.
+      apply IHatomic_exec2; eauto.
+  Qed.
+
+  Lemma exec_tid_disjoint_reads : forall tid0 v tid1 T s p s' result' evs,
+    tid0 <> tid1 ->
+    @exec_tid opT opHiT State op_step T tid1 s p s' result' evs ->
+    @exec_tid opT opHiT State op_step T tid1 (state_upd s tid0 v) p (state_upd s' tid0 v) result' evs.
+  Proof.
+    intros.
+    induction H0; simpl; eauto.
+    constructor.
+    induction H0; eauto.
+  Qed.
+
+  Theorem hitrace_incl_s_op_step :
+    forall AT (ap : proc opT opHiT AT) T (rx : AT -> proc _ _ T) s s' r tid evs,
+      atomic_exec op_step ap tid s r s' evs ->
+      trace_match_hi (prepend tid evs TraceEmpty) TraceEmpty ->
+      hitrace_incl_s s s' tid
+        op_step (Bind (Atomic ap) rx) (rx r).
+  Proof.
+    intros.
+
+    induction H; simpl in *; intros;
+      match goal with
+      | H : trace_match_hi _ _ |- _ =>
+        try solve [ inversion H ]
+      end.
+
+    admit.
+
+    eapply hitrace_incl_s_trans.
+    eapply IHatomic_exec1.
+
+XXX
+
+    (forall s tid r s' evs,
+      atomic_exec op_step (Atomic skew_proc) tid s r s' evs ->
+      s' = skew_effect s tid) ->
+    (forall s tid r s',
+      op_step op tid s r s' ->
+      r = op_ret s tid /\
+      s' = op_effect s tid) ->
+    (forall r s tid, hitrace_incl_s s (skew_effect s tid) tid op_step (p1 r) (p2 r)) ->
+    forall s tid,
+    hitrace_incl_s s (skew_effect (op_effect s tid) tid) tid
+      op_step (r <- OpExec op; p1 r) (p2 (op_ret s tid)).
+
+
+
+    forall ST (skew_proc : proc opT opHiT ST)
+           (skew_effect : State -> nat -> State)
+           (op_effect : State -> nat -> State)
+           (op_ret : State -> nat -> T'),
+    (forall s tid r s' evs,
+      atomic_exec op_step (Atomic skew_proc) tid s r s' evs ->
+      s' = skew_effect s tid) ->
+    (forall s tid r s',
+      op_step op tid s r s' ->
+      r = op_ret s tid /\
+      s' = op_effect s tid) ->
+    (forall r s tid, hitrace_incl_s s (skew_effect s tid) tid op_step (p1 r) (p2 r)) ->
+    forall s tid,
+    hitrace_incl_s s (skew_effect (op_effect s tid) tid) tid
+      op_step (r <- OpExec op; p1 r) (p2 (op_ret s tid)).
+  Proof.
+    unfold hitrace_incl_s, hitrace_incl_ts_s; intros.
+
+    match goal with
+    | H : exec _ _ (thread_upd ?ts ?tid ?p) _ |- _ =>
+      remember (thread_upd ts tid p);
+      generalize dependent ts;
+      induction H; intros; subst
+    end.
+
+    - destruct (tid0 == tid); subst.
+      + autorewrite with t in *.
+        repeat maybe_proc_inv.
+        repeat exec_tid_inv.
+        edestruct H1; eauto.
+        eexists; intuition eauto.
+
+        eapply H in H8 as H8'; intuition subst.
+
+      + edestruct IHexec.
+        rewrite thread_upd_upd_ne; eauto.
+        intuition idtac.
+
+        eexists; split.
+        eapply ExecOne with (tid := tid0).
+          autorewrite with t in *; eauto.
+          eapply exec_tid_disjoint_reads; eauto.
+          rewrite thread_upd_upd_ne; eauto.
+          erewrite exec_tid_disjoint_writes with (s := s) (tid1 := tid);
+            eauto.
+        eauto.
+
+    - exfalso; eauto.
+  Qed.
+
+End Disjoint.
